remove equivalence.dfy and move content

src/Distributions/UniformPowerOfTwo/Model.dfy
@@ -10,6 +10,11 @@ module UniformPowerOfTwo.Model {
   import Monad
   import Independence
   import Loops
+  import NatArith
+
+  /************
+   Definitions
+  ************/
 
   // Adapted from Definition 48 (see issue #79 for the reason of the modification)
   // The return value u is uniformly distributed between 0 <= u < 2^k where 2^k <= n < 2^(k + 1).
@@ -29,5 +34,127 @@ module UniformPowerOfTwo.Model {
 
   function UnifStep(m: nat): Monad.Hurd<nat> {
     Monad.Bind(Monad.Coin, UnifStepHelper(m))
+  }
+
+
+  // A tail recursive version of Sample
+  function SampleTailRecursive(n: nat, u: nat := 0): Monad.Hurd<nat>
+    requires n >= 1
+  {
+    (s: Rand.Bitstream) =>
+      if n == 1 then
+        Monad.Result(u, s)
+      else
+        SampleTailRecursive(n / 2, if Rand.Head(s) then 2*u + 1 else 2*u)(Rand.Tail(s))
+  }
+
+  /*******
+   Lemmas
+  *******/
+
+  // Equivalence of Sample and its tail-recursive version
+  lemma SampleCorrespondence(n: nat, s: Rand.Bitstream)
+    requires n >= 1
+    ensures SampleTailRecursive(n)(s) == Sample(n)(s)
+  {
+    if n == 1 {
+      reveal Sample();
+      assert SampleTailRecursive(n)(s) == Sample(n)(s);
+    } else {
+      var k := NatArith.Log2Floor(n);
+      assert NatArith.Power(2, k) <= n < NatArith.Power(2, k + 1) by { NatArith.Power2OfLog2Floor(n); }
+      calc {
+        SampleTailRecursive(n)(s);
+        { SampleTailRecursiveEqualIfSameLog2Floor(n, NatArith.Power(2, k), k, 0, s); }
+        SampleTailRecursive(NatArith.Power(2, k))(s);
+        Monad.Bind(Sample(NatArith.Power(2, 0)), (u: nat) => SampleTailRecursive(NatArith.Power(2, k), u))(s);
+        { RelateWithTailRecursive(k, 0, s); }
+        Sample(NatArith.Power(2, k))(s);
+        { SampleEqualIfSameLog2Floor(n, NatArith.Power(2, k), k, s); }
+        Sample(n)(s);
+      }
+    }
+  }
+
+  // All numbers between consecutive powers of 2 behave the same as arguments to SampleTailRecursive
+  lemma SampleTailRecursiveEqualIfSameLog2Floor(m: nat, n: nat, k: nat, u: nat, s: Rand.Bitstream)
+    requires m >= 1
+    requires n >= 1
+    requires NatArith.Power(2, k) <= m < NatArith.Power(2, k + 1)
+    requires NatArith.Power(2, k) <= n < NatArith.Power(2, k + 1)
+    ensures SampleTailRecursive(m, u)(s) == SampleTailRecursive(n, u)(s)
+  {
+    if k == 0 {
+      assert m == n;
+    } else {
+      assert 1 <= m;
+      assert 1 <= n;
+      calc {
+        SampleTailRecursive(m, u)(s);
+        SampleTailRecursive(m / 2, if Rand.Head(s) then 2*u + 1 else 2*u)(Rand.Tail(s));
+        { SampleTailRecursiveEqualIfSameLog2Floor(m / 2, n / 2, k - 1, if Rand.Head(s) then 2*u + 1 else 2*u, Rand.Tail(s)); }
+        SampleTailRecursive(n / 2, if Rand.Head(s) then 2*u + 1 else 2*u)(Rand.Tail(s));
+        SampleTailRecursive(n, u)(s);
+      }
+    }
+  }
+
+  // All numbers between consecutive powers of 2 behave the same as arguments to Sample
+  lemma SampleEqualIfSameLog2Floor(m: nat, n: nat, k: nat, s: Rand.Bitstream)
+    requires m >= 1
+    requires n >= 1
+    requires NatArith.Power(2, k) <= m < NatArith.Power(2, k + 1)
+    requires NatArith.Power(2, k) <= n < NatArith.Power(2, k + 1)
+    ensures Sample(m)(s) == Sample(n)(s)
+  {
+    if k == 0 {
+      assert m == n;
+    } else {
+      assert 1 <= m;
+      assert 1 <= n;
+      calc {
+        Sample(m)(s);
+        { reveal Sample(); }
+        Monad.Bind(Sample(m / 2), UnifStep)(s);
+        { SampleEqualIfSameLog2Floor(m / 2, n / 2, k - 1, s); }
+        Monad.Bind(Sample(n / 2), UnifStep)(s);
+        { reveal Sample(); }
+        Sample(n)(s);
+      }
+    }
+  }
+
+  // The induction invariant for the equivalence proof (generalized version of SampleCorrespondence)
+  lemma RelateWithTailRecursive(l: nat, m: nat, s: Rand.Bitstream)
+    decreases l
+    ensures Monad.Bind(Sample(NatArith.Power(2, m)), (u: nat) => SampleTailRecursive(NatArith.Power(2, l), u))(s) == Sample(NatArith.Power(2, m + l))(s)
+  {
+    if l == 0 {
+      calc {
+        Monad.Bind(Sample(NatArith.Power(2, m)), (u: nat) => SampleTailRecursive(NatArith.Power(2, l), u))(s);
+        (var Result(u, s') := Sample(NatArith.Power(2, m))(s); SampleTailRecursive(1, u)(s'));
+        Sample(NatArith.Power(2, m + l))(s);
+      }
+    } else {
+      assert LGreaterZero: NatArith.Power(2, l) >= 1 by { NatArith.PowerGreater0(2, l); }
+      assert MGreaterZero: NatArith.Power(2, m) >= 1 by { NatArith.PowerGreater0(2, m); }
+      assert L1GreaterZero: NatArith.Power(2, l - 1) >= 1 by { NatArith.PowerGreater0(2, l - 1); }
+      calc {
+        Monad.Bind(Sample(NatArith.Power(2, m)), (u: nat) => SampleTailRecursive(NatArith.Power(2, l), u))(s);
+        (var Result(u, s') := Sample(NatArith.Power(2, m))(s); SampleTailRecursive(NatArith.Power(2, l), u)(s'));
+        { reveal LGreaterZero; }
+        (var Result(u, s') := Sample(NatArith.Power(2, m))(s);
+         SampleTailRecursive(NatArith.Power(2, l) / 2, if Rand.Head(s') then 2 * u + 1 else 2 * u)(Rand.Tail(s')));
+        { assert NatArith.Power(2, l) / 2 == NatArith.Power(2, l - 1); reveal L1GreaterZero; }
+        (var Result(u', s') := Monad.Bind(Sample(NatArith.Power(2, m)), UnifStep)(s);
+         SampleTailRecursive(NatArith.Power(2, l - 1), u')(s'));
+        { assert NatArith.Power(2, m + 1) / 2 == NatArith.Power(2, m); reveal Sample(); }
+        (var Result(u', s') := Sample(NatArith.Power(2, m + 1))(s);
+         SampleTailRecursive(NatArith.Power(2, l - 1), u')(s'));
+        Monad.Bind(Sample(NatArith.Power(2, m + 1)), (u: nat) => SampleTailRecursive(NatArith.Power(2, l - 1), u))(s);
+        { RelateWithTailRecursive(l - 1, m + 1, s); }
+        Sample(NatArith.Power(2, m + l))(s);
+      }
+    }
   }
 }
